theories/νSet/Equiv/Face.v
@@ -17,6 +17,8 @@ Set Warnings "-notation-overridden".
 From Bonak Require Import SigT HSet LeSProp Notation νSet.Layer νSet.
 From Bonak Require νSetEquiv.
 
+From Bonak Require Import Limit.
+
 Set Primitive Projections.
 Set Printing Projections.
 Set Keyed Unification.
